src/unitb/models/nondet.lean
@@ -26,7 +26,7 @@ structure event : Type :=
 parameter {α}
 
 def event.guard (e : event) : pred :=
-e.coarse_sch && e.fine_sch
+e.coarse_sch ⋀ e.fine_sch
 
 parameter α
 
@@ -59,7 +59,7 @@ def program.init (s : program) (p : pred) : Prop :=
 s^.first ⟹ p
 
 def program.guard  (s : program) (e : option s.lbl) : α → Prop :=
-(s^.event e)^.coarse_sch && (s^.event e)^.fine_sch
+(s^.event e)^.coarse_sch ⋀ (s^.event e)^.fine_sch
 
 def program.guard_none_holds (s : program) (σ : α)
 : s.guard none σ :=
@@ -122,7 +122,7 @@ begin
 end
 
 lemma is_step_exists_event  (s : program)
- : temporal.action (is_step s) = (⟦ eq ⟧ || ∃∃ ev : s.lbl, ⟦ (s.event' ev).step_of ⟧) :=
+ : temporal.action (is_step s) = (⟦ eq ⟧ ⋁ ∃∃ ev : s.lbl, ⟦ (s.event' ev).step_of ⟧) :=
 begin
   simp [exists_action,or_action],
   apply congr_arg,
@@ -198,7 +198,7 @@ def program.transient (s : program) (p q : pred' α) : Prop :=
 open temporal has_mem scheduling.unitb function
 
 lemma object_mch_action_eq_step_of (s : program) (e : option s.lbl)
-: •mem e ∘ s.object_mch.req && action (s.object_mch.action e) ⟹ action (s.step_of e) :=
+: •mem e ∘ s.object_mch.req ⋀ action (s.object_mch.action e) ⟹ action (s.step_of e) :=
 begin
   rw [init_eq_action,action_and_action],
   apply action_entails_action,
@@ -215,13 +215,13 @@ begin
 end
 
 lemma mem_object_req_eq_csch_and_fsch (s : program) (e : option s.lbl)
-: mem e ∘ s.object_mch.req = s.coarse_sch_of e && s.fine_sch_of e :=
+: mem e ∘ s.object_mch.req = s.coarse_sch_of e ⋀ s.fine_sch_of e :=
 rfl
 
 lemma program.falsify.negate
    {s : program} {act : option s.lbl} {p q : pred}
 :  s.falsify act p q
-→  •q && ⟦ s^.step_of act ⟧ ⟹ <>-•q :=
+→  •q ⋀ ⟦ s^.step_of act ⟧ ⟹ ◇-•q :=
 begin
   intros h₀ τ h₁,
   have h₂ := h₀.negate' _ h₁.left h₁.right,
@@ -263,11 +263,11 @@ begin
   { apply entails_trans _ hp h'.schedule, },
   { have hp' := init_entails_init hp,
     have hq' := init_entails_init hq,
-    apply ew_imp_ew _ h'.negate',
-    apply p_imp_entails_p_imp hq' _,
-    apply p_imp_entails_p_imp_right _,
-    apply next_imp_next _ ,
-    apply p_not_entails_p_not_right hq', }
+    apply' ew_imp_ew _ h'.negate',
+    refine p_imp_entails_p_imp hq' _,
+    refine p_imp_entails_p_imp_right _,
+    apply' next_imp_next _ ,
+    apply' p_not_entails_p_not_right hq', }
 end
 
 end theorems
@@ -283,9 +283,9 @@ instance prog_is_system : unitb.system program :=
 section soundness
 
 def fair' (s : program) (e : option s.lbl) (τ : stream α) : Prop :=
-(<>[]• s^.coarse_sch_of e) τ →
-([]<>•s.fine_sch_of e) τ →
-([]<>⟦ s.step_of e ⟧) τ
+(◇◻• s^.coarse_sch_of e) τ →
+(◻◇•s.fine_sch_of e) τ →
+(◻◇⟦ s.step_of e ⟧) τ
 
 structure program.ex (s : program) (τ : stream α) : Prop :=
     (init : s^.first (τ 0))
@@ -300,16 +300,16 @@ variables (τ : stream α)
 lemma transient.semantics'
   (h : ∀ e, fair' s e τ)
   (T₀ : s.transient p q)
-: ([]<>•p) τ → ([]<>-•q) τ :=
+: (◻◇•p) τ → (◻◇-•q) τ :=
 begin
   cases (temporal.em' (•q) τ) with h_q ev_nq,
   { dunfold nondet.program.transient at T₀,
     cases T₀ with ev T₀,
-    have Hc : (<>[]•s.coarse_sch_of ev) τ,
+    have Hc : (◇◻•s.coarse_sch_of ev) τ,
     { apply stable_entails_stable' _ _ h_q,
       apply T₀.enable },
     intro Hp,
-    have Hf : ([]<>•s.fine_sch_of ev) τ,
+    have Hf : (◻◇•s.fine_sch_of ev) τ,
     { apply inf_often_entails_inf_often' _ _ Hp,
       apply T₀.schedule, },
     have live := h ev Hc Hf,
@@ -335,7 +335,7 @@ end
 
 lemma transient.semantics
   (T₀ : s.transient p q)
-: ([]<>•p) τ → ([]<>-•q) τ :=
+: (◻◇•p) τ → (◻◇-•q) τ :=
 nondet.transient.semantics' τ h.liveness T₀
 
 end soundness
@@ -355,17 +355,18 @@ begin
   { rw h.init,
     apply classical.some_spec },
   { unfold saf_ex,
-    apply henceforth_entails_henceforth _ _ h.valid,
+    revert_p h.valid, monotonicity,
     rw p_exists_entails_eq_p_forall_entails,
     intro l,
     intros τ h,
     apply is_step_inst' _ l,
     apply object_mch_action_eq_step_of,
-    revert h, apply and.imp_left _,
-    apply id, },
-  { apply forall_imp_forall _ h.fair,
-    intros e Hsch Hc Hf,
-    apply inf_often_entails_inf_often (object_mch_action_eq_step_of _ _),
+    revert_p h, refl },
+  { have h' := h.fair, revert h',
+    intros_mono e,
+    intros Hsch Hc Hf,
+    apply inf_often_entails_inf_often,
+    apply (object_mch_action_eq_step_of _ _),
     apply Hsch,
     rw mem_object_req_eq_csch_and_fsch,
     apply coincidence Hc Hf },
@@ -442,8 +443,8 @@ begin
 end
 
 theorem ensure_rule {s : program} {p q : pred' α} (ev : option s.lbl)
-   (EN : p && -q ⟹ s.coarse_sch_of ev)
-   (FLW : p && -q && s.coarse_sch_of ev  ↦  s.fine_sch_of ev || q in s)
+   (EN : p ⋀ -q ⟹ s.coarse_sch_of ev)
+   (FLW : p ⋀ -q ⋀ s.coarse_sch_of ev  ↦  s.fine_sch_of ev ⋁ q in s)
    (NEG : ∀ σ σ', ¬ q σ → s.step_of ev σ σ' → q σ')
    (STABLE: unless s p q )
 : p ↦ q in s :=
