src/unitb/refinement/split_merge.lean
@@ -18,9 +18,9 @@ structure evt_ref (lbl : Type) (mc : program α) (ea : event α) (ecs : lbl → 
   (witness : lbl → α → Prop)
   (witness_fis : ⦃ ∃∃ e, witness e ⦄)
   (sim : ∀ ec, ⟦ (ecs ec).step_of ⟧ ⟹ ⟦ ea.step_of ⟧)
-  (delay : ∀ ec, witness ec && ea.coarse_sch && ea.fine_sch ↦ witness ec && (ecs ec).coarse_sch in mc)
-  (stable : ∀ ec, unless_except mc (witness ec && (ecs ec).coarse_sch) (-ea.coarse_sch) { e | ∃ l, ecs l = e })
-  (resched : ∀ ec, ea.coarse_sch && ea.fine_sch && witness ec ↦ (ecs ec).fine_sch in mc)
+  (delay : ∀ ec, witness ec ⋀ ea.coarse_sch ⋀ ea.fine_sch ↦ witness ec ⋀ (ecs ec).coarse_sch in mc)
+  (stable : ∀ ec, unless_except mc (witness ec ⋀ (ecs ec).coarse_sch) (-ea.coarse_sch) { e | ∃ l, ecs l = e })
+  (resched : ∀ ec, ea.coarse_sch ⋀ ea.fine_sch ⋀ witness ec ↦ (ecs ec).fine_sch in mc)
 
 structure refined (ma mc : program α) : Type :=
   (sim_init : mc^.first ⟹ ma^.first)
@@ -67,16 +67,16 @@ def W (e' : imp_lbl) := (R.events e).witness e'
 def CC (e' : option mc.lbl) := mc.coarse_sch_of e'
 def CF (e' : option mc.lbl) := mc.fine_sch_of e'
 
-parameter abs_coarse : (<>[](•AC && -⟦ ma.step_of e ⟧)) τ
+parameter abs_coarse : (◇◻(•AC ⋀ -⟦ ma.step_of e ⟧)) τ
 
-parameter abs_fine : ([]<>•AF) τ
+parameter abs_fine : (◻◇•AF) τ
 
 include M₁
 include abs_coarse
 include abs_fine
 
 lemma abs_coarse_and_fine
-: ([]<>(•AC && •AF)) τ :=
+: (◻◇(•AC ⋀ •AF)) τ :=
 begin
   apply coincidence,
   { apply stable_entails_stable _ _ abs_coarse,
@@ -84,10 +84,10 @@ begin
   { apply abs_fine },
 end
 
-lemma conc_coarse : ∃ e', (<>[](• W e' && • CC e'.val) ) τ :=
+lemma conc_coarse : ∃ e', (◇◻(• W e' ⋀ • CC e'.val) ) τ :=
 begin
-  have H : ((∃∃ e', <>[](• W ma mc R e e' && • CC mc e'.val))
-                   || []<>((-•AC ma e) || ∃∃ e' : imp_lbl ma mc R e, ⟦ mc.step_of e'.val ⟧)) τ,
+  have H : ((∃∃ e', ◇◻(• W ma mc R e e' ⋀ • CC mc e'.val))
+                   ⋁ ◻◇((-•AC ma e) ⋁ ∃∃ e' : imp_lbl ma mc R e, ⟦ mc.step_of e'.val ⟧)) τ,
   { rw exists_action,
     apply p_or_p_imp_p_or_right _ (unless_sem_exists' M₁.safety (R.events e).stable _),
     { apply inf_often_entails_inf_often,
@@ -124,8 +124,8 @@ begin
 end
 
 lemma conc_fine : ∀ e',
-         (<>[]•W e') τ →
-         ([]<>•CF e'.val) τ :=
+         (◇◻•W e') τ →
+         (◻◇•CF e'.val) τ :=
 begin
   intros e' H,
   have H' := system_sem.leads_to_sem ((R.events e).resched e') _ M₁,
@@ -150,15 +150,15 @@ begin
     apply M₁.safety },
   { intros e COARSE₀ FINE₀,
     apply assume_neg _, intro ACT,
-    have COARSE₁ :  (<>[](•AC ma e && -⟦program.step_of ma e⟧)) τ,
+    have COARSE₁ :  (◇◻(•AC ma e ⋀ -⟦program.step_of ma e⟧)) τ,
     { rw [p_not_eq_not,not_henceforth,not_eventually] at ACT,
       apply stable_and_of_stable_of_stable COARSE₀ ACT },
     clear COARSE₀ ACT,
     cases conc_coarse ma mc R τ M₁ _ COARSE₁ FINE₀ with e' C_COARSE',
-    have C_COARSE : (<>[]•CC mc e'.val) τ,
+    have C_COARSE : (◇◻•CC mc e'.val) τ,
     { apply stable_entails_stable _ _ C_COARSE',
       intro, apply and.right },
-    have WIT : (<>[]•W ma mc R e e') τ,
+    have WIT : (◇◻•W ma mc R e e') τ,
     { apply stable_entails_stable _ _ C_COARSE',
       intro, apply and.left },
     have C_FINE := conc_fine ma mc R τ M₁ e COARSE₁ FINE₀ e' WIT,
